HouLean/OpenCL/Compiler/Types2.lean
@@ -1,0 +1,22 @@
+import HouLean.OpenCL.Compiler.RewriteRules
+import HouLean.OpenCL.Compiler.Grammar2
+
+open Lean Meta Simp
+
+namespace HouLean.OpenCL.Compiler3
+
+structure Context where
+  fvarMap : ExprMap String := {}
+  usedNames : Std.HashMap String Nat := {}
+
+structure State where
+  statements : Array (TSyntax `clStmtLike) := #[]
+  -- all functions that has been compiled in this run
+
+abbrev CompileM := ReaderT Context <| StateT State <| MetaM
+
+initialize compileFunctionRef : IO.Ref (Expr → CompileM (TSyntax `clFunction)) ←
+  IO.mkRef (fun _ => pure default)
+
+def compileFunction (f : Expr) : CompileM (TSyntax `clFunction) := do
+  (← compileFunctionRef.get) f
