HouLean/OpenCL/Reference/DataTypes.lean
@@ -1,11 +1,12 @@
 import HouLean.OpenCL.Compiler.RewriteRules
+import HouLean.OpenCL.Compiler.Main2
+import HouLean.OpenCL.Basic
 
-open Lean HouLean Meta OpenCL Compiler Compiler3 Math
+open Lean HouLean Meta OpenCL Compiler2 Math
 
 namespace HouLean.OpenCL
 
 variable {α : Type} [AtomicOpenCLType α] {n : Nat}
-
 
 
 ----------------------------------------------------------------------------------------------------
@@ -43,9 +44,10 @@ impl_by {n : Nat} {T} [AtomicOpenCLType T] [AllowedVectorSize n] : Vector T n ==
 
   let name := mkIdent <| type.getId.appendAfter (toString n)
 
-  return ← `(oclExpr| $name:ident)
+  return ← `(clExpr| $name:ident)
 
 
+open Compiler2 in
 /- Vector contructor rule  e.g. #v[x,y,z] ==> (float3){x,y,z}
 
 The notation `#v[x,y,z]` stands for `Vector.mk [x,y,z].toArray h` and this rule matches on this
@@ -63,4 +65,4 @@ impl_by {n : Nat} {α : Type} [AtomicOpenCLType α] [AllowedVectorSize n] (l : L
     | throwError m!"Size {n} of vector has to be known at compile time!"
   let name := mkIdent <| type.getId.appendAfter (toString n)
 
-  return ← `(oclExpr| ($name){$xs:oclExpr,*} )
+  return ← `(clExpr| ($name){$[$xs:clExpr],*} )
