Tests/OpenCL/Compiler2.lean
@@ -1,0 +1,65 @@
+import HouLean.OpenCL.Compiler
+import HouLean.OpenCL.Reference
+
+open HouLean.OpenCL Compiler2
+
+namespace Test.OpenCL.Compiler2
+
+
+
+open Lean Elab Term Meta in
+elab c:"#ocl_compile" f:term : command => do
+  Command.runTermElabM fun _ => do
+    let f ← elabTermAndSynthesize f none
+    lambdaTelescope f fun _ b => do
+      let (_,s) ← compileBlock b {} {}
+      let stx ← `(clCompStmt| { $s.statements* })
+      logInfoAt c stx
+
+
+
+/--
+info: {
+      double a = x * y;
+      return a + x * y;
+}
+-/
+#guard_msgs in
+#ocl_compile fun x y : Float =>
+  let a := x * y
+  a + x * y
+
+/--
+info: {
+      double a = x * y;
+      double b = a - x + y;
+      return a + x * y / b;
+}
+-/
+#guard_msgs in
+#ocl_compile fun x y : Float =>
+  let a := x * y
+  let b := a - x + y
+  a + x * y / b
+
+
+def foo (x y : Float) :=
+  let a := x * y
+  let b := a - x + y
+  a + x * y / b
+
+run_meta
+  compileDecl ``foo
+
+#ocl_compile fun x y : Float => foo x y
+
+
+-- open Lean Meta Qq
+-- run_meta
+--   let t ← compileType q(Nat × Float)
+--   logInfo m!"{t}"
+
+-- open Lean Meta Qq
+-- run_meta
+--   let t ← compileType q(Vector (Vector (Vector Float32 4) 4) 4)
+--   logInfo m!"{t}"
